More WIP for chacha, try further with effect layering

examples/steel_wip/chacha20/Steel.Impl.Chacha20.fst
@@ -22,8 +22,9 @@ val rounds: st:state -> RST unit
 // #set-options "--z3cliopt smt.qi.eager_threshold=100"
 // #set-options "--query_stats"
 
+module HST = FStar.HyperStack.ST
+
 let rounds st =
-  let h0 = get (A.array_resource st) in
   double_round st;
   double_round st;
   double_round st;
@@ -33,11 +34,7 @@ let rounds st =
   double_round st;
   double_round st;
   double_round st;
-  double_round st;
-  let h1 = get (A.array_resource st) in
-  assert (P.allows_write (A.get_rperm st h1));
-  assert (A.as_rseq st h1 == Spec.rounds (A.as_rseq st h0));
-  admit()
+  double_round st
 
 val chacha20_core:
     k:state
@@ -53,9 +50,129 @@ val chacha20_core:
     A.as_rseq k h1 == Spec.chacha20_core ctr (A.as_rseq ctx0 h0))
 
 let chacha20_core k ctx ctr =
-  admit()
-  // copy_state k ctx;
-  // k.(12ul) <- k.(12ul) +. ctr_u32;
-  // rounds k;
-  // sum_state k ctx;
-  // k.(12ul) <- k.(12ul) +. ctr_u32
+  copy_state k ctx;
+  let v = rst_frame
+    (A.array_resource k <*> A.array_resource ctx)
+    (fun _ -> A.array_resource k <*> A.array_resource ctx)
+    (fun _ -> A.index k 12ul) `UInt32.add_mod` ctr
+  in
+  rst_frame
+    (A.array_resource k <*> A.array_resource ctx)
+    (fun _ -> A.array_resource k <*> A.array_resource ctx)
+    (fun _ -> A.upd k 12ul v);
+  rst_frame
+    (A.array_resource k <*> A.array_resource ctx)
+    (fun _ -> A.array_resource k <*> A.array_resource ctx)
+    (fun _ -> rounds k);
+  sum_state k ctx;
+  let v = rst_frame
+    (A.array_resource k <*> A.array_resource ctx)
+    (fun _ -> A.array_resource k <*> A.array_resource ctx)
+    (fun _ -> A.index k 12ul) `UInt32.add_mod` ctr
+  in
+  rst_frame
+    (A.array_resource k <*> A.array_resource ctx)
+    (fun _ -> A.array_resource k <*> A.array_resource ctx)
+    (fun _ -> A.upd k 12ul v)
+
+val setup:
+    st:state
+  -> k:A.array UInt8.t{A.vlength k == 32}
+  -> n:A.array UInt8.t{A.vlength k == 12}
+  -> ctr0:Spec.counter ->
+  RST unit
+  (A.array_resource st <*> A.array_resource k <*> A.array_resource n)
+  (fun _ -> A.array_resource st <*> A.array_resource k <*> A.array_resource n)
+  (requires fun h -> P.allows_write (A.get_rperm st h))
+  (ensures  fun h0 _ h1 ->
+    h0 (A.array_resource k) == h1 (A.array_resource k) /\
+    h0 (A.array_resource n) == h1 (A.array_resource n) /\
+    P.allows_write (A.get_rperm st h1) /\
+    A.as_rseq st h1 `Seq.equal` Spec.setup (A.as_rseq k h0) (A.as_rseq n h0) ctr0 (A.as_rseq st h0))
+
+let setup st k n ctr0 =
+  rst_frame
+    (A.array_resource st <*> A.array_resource k <*> A.array_resource n)
+    (fun _ -> A.array_resource st <*> A.array_resource k <*> A.array_resource n)
+    (fun _ -> A.upd st 0ul Spec.c0);
+  rst_frame
+    (A.array_resource st <*> A.array_resource k <*> A.array_resource n)
+    (fun _ -> A.array_resource st <*> A.array_resource k <*> A.array_resource n)
+    (fun _ -> A.upd st 1ul Spec.c1);
+  rst_frame
+    (A.array_resource st <*> A.array_resource k <*> A.array_resource n)
+    (fun _ -> A.array_resource st <*> A.array_resource k <*> A.array_resource n)
+    (fun _ -> A.upd st 2ul Spec.c2);
+  rst_frame
+    (A.array_resource st <*> A.array_resource k <*> A.array_resource n)
+    (fun _ -> A.array_resource st <*> A.array_resource k <*> A.array_resource n)
+    (fun _ -> A.upd st 3ul Spec.c3);
+
+  let st04, st416 =
+    rst_frame
+      (A.array_resource st <*> A.array_resource k <*> A.array_resource n)
+      (fun v -> A.array_resource (fst v) <*> A.array_resource (snd v) <*> A.array_resource k <*> A.array_resource n)
+      (fun _ -> A.split st 4ul) in
+  let st48, st816 =
+    rst_frame
+      (A.array_resource st04 <*> A.array_resource st416 <*> A.array_resource k <*> A.array_resource n)
+      (fun v -> A.array_resource (fst v) <*> A.array_resource (snd v) <*> A.array_resource st04 <*> A.array_resource k <*> A.array_resource n)
+      (fun _ -> A.split st416 4ul) in
+
+  rst_frame
+    (A.array_resource st48 <*> A.array_resource st816 <*> A.array_resource st04 <*> A.array_resource k <*> A.array_resource n)
+    (fun _ -> A.array_resource st48 <*> A.array_resource st816 <*> A.array_resource st04 <*> A.array_resource k <*> A.array_resource n)
+    (fun _ -> uints_from_bytes_le #4 st48 k);
+
+  rst_frame
+    (A.array_resource st48 <*> A.array_resource st816 <*> A.array_resource st04 <*> A.array_resource k <*> A.array_resource n)
+    (fun _ -> A.array_resource st416 <*> A.array_resource st04 <*> A.array_resource k <*> A.array_resource n)
+    (fun _ -> A.glue st416 st48 st816);
+
+  rst_frame
+    (A.array_resource st416 <*> A.array_resource st04 <*> A.array_resource k <*> A.array_resource n)
+    (fun _ -> A.array_resource st <*> A.array_resource k <*> A.array_resource n)
+    (fun _ -> A.glue st st04 st416);
+
+  rst_frame
+    (A.array_resource st <*> A.array_resource k <*> A.array_resource n)
+    (fun _ -> A.array_resource st <*> A.array_resource k <*> A.array_resource n)
+    (fun _ -> A.upd st 12ul ctr0);
+
+  let st013, st1316 =
+    rst_frame
+      (A.array_resource st <*> A.array_resource k <*> A.array_resource n)
+      (fun v -> A.array_resource (fst v) <*> A.array_resource (snd v) <*> A.array_resource k <*> A.array_resource n)
+      (fun _ -> A.split st 13ul) in
+
+  rst_frame
+    (A.array_resource st013 <*> A.array_resource st1316 <*> A.array_resource k <*> A.array_resource n)
+    (fun _ -> A.array_resource st013 <*> A.array_resource st1316 <*> A.array_resource k <*> A.array_resource n)
+    (fun _ -> uints_from_bytes_le #4 st1316 n);
+
+  rst_frame
+    (A.array_resource st013 <*> A.array_resource st1316 <*> A.array_resource k <*> A.array_resource n)
+    (fun _ -> A.array_resource st <*> A.array_resource k <*> A.array_resource n)
+    (fun _ -> A.glue st st013 st1316)
+
+val chacha20_init:
+     k:A.array UInt8.t{A.vlength k == 32}
+  -> n:A.array UInt8.t{A.vlength k == 12}
+  -> ctr0:Spec.counter ->
+  RST state
+  (A.array_resource k <*> A.array_resource n)
+  (fun st -> A.array_resource st <*> A.array_resource k <*> A.array_resource n)
+  (requires fun h -> True)
+  (ensures  fun h0 st h1 ->
+    h0 (A.array_resource k) == h1 (A.array_resource k) /\
+    h0 (A.array_resource n) == h1 (A.array_resource n) /\
+    P.allows_write (A.get_rperm st h1) /\
+    A.as_rseq st h1 == Spec.chacha20_init (A.as_rseq k h0) (A.as_rseq n h0) ctr0)
+
+let chacha20_init k n ctr0 =
+  let st = rst_frame
+    (A.array_resource k <*> A.array_resource n)
+    (fun st -> A.array_resource st <*> A.array_resource k <*> A.array_resource n)
+    (fun _ -> A.alloc 0ul 16ul) in
+  setup st k n ctr0;
+  st
