examples/steel_wip/chacha20/Steel.Impl.Chacha20.Core32.fsti
@@ -1,0 +1,142 @@
+module Steel.Impl.Chacha20.Core32
+
+open Steel.RST
+open FStar.UInt32
+module A = Steel.Array
+module P = LowStar.Permissions
+
+module Spec = Steel.Spec.Chacha20
+
+let state = b:A.array t{A.vlength b == 16}
+let index = i:UInt32.t{v i < 16}
+let size = Spec.size
+
+val create_state: unit -> RST state
+  (empty_resource)
+  (fun st -> A.array_resource st)
+  (fun _ -> True)
+  (fun _ st h1 ->
+      A.freeable st /\
+      A.as_rseq st h1 == Seq.create 16 0ul /\
+      A.get_rperm st h1 = FStar.Real.one)
+
+val line:
+  st:state
+  -> a:index
+  -> b:index
+  -> d:index
+  -> r:Spec.rotval ->
+  RST unit
+    (A.array_resource st)
+    (fun _ -> A.array_resource st)
+    (requires fun h0 -> v a <> v d /\ P.allows_write (A.get_rperm st h0))
+    (ensures fun h0 _ h1 ->
+      P.allows_write (A.get_rperm st h1) /\
+      A.as_rseq st h1 == Spec.line (v a) (v b) (v d) r (A.as_rseq st h0))
+
+val quarter_round:
+    st:state
+  -> a:index
+  -> b:index
+  -> c:index
+  -> d:index ->
+  RST unit
+  (A.array_resource st)
+  (fun _ -> A.array_resource st)
+  (requires fun h -> v a <> v d /\ v c <> v b /\
+    P.allows_write (A.get_rperm st h))
+  (ensures  fun h0 _ h1 ->
+    P.allows_write (A.get_rperm st h1) /\
+    A.as_rseq st h1 == Spec.quarter_round (v a) (v b) (v c) (v d) (A.as_rseq st h0))
+
+val double_round:
+  st:state ->
+  RST unit
+  (A.array_resource st)
+  (fun _ -> A.array_resource st)
+  (requires fun h -> P.allows_write (A.get_rperm st h))
+  (ensures  fun h0 _ h1 ->
+    P.allows_write (A.get_rperm st h1) /\
+    A.as_rseq st h1 == Spec.double_round (A.as_rseq st h0))
+
+inline_for_extraction
+val copy_state:
+    st:state
+  -> ost:state ->
+  RST unit
+  (A.array_resource st <*> A.array_resource ost)
+  (fun _ -> A.array_resource st <*> A.array_resource ost)
+  (requires fun h -> P.allows_write (A.get_rperm st h))
+  (ensures  fun h0 _ h1 ->
+    h0 (A.array_resource ost) == h1 (A.array_resource ost) /\
+    P.allows_write (A.get_rperm st h1) /\
+    A.as_rseq st h1 `Seq.equal` A.as_rseq ost h0)
+
+val sum_state:
+    st:state
+  -> ost:state ->
+  RST unit
+  (A.array_resource st <*> A.array_resource ost)
+  (fun _ -> A.array_resource st <*> A.array_resource ost)
+  (requires fun h -> P.allows_write (A.get_rperm st h))
+  (ensures  fun h0 _ h1 ->
+    h0 (A.array_resource ost) == h1 (A.array_resource ost) /\
+    P.allows_write (A.get_rperm st h1) /\
+    A.as_rseq st h1 `Seq.equal` Spec.sum_state (A.as_rseq st h0) (A.as_rseq ost h0))
+
+open FStar.Mul
+
+val uints_from_bytes_le:  #len:nat
+  -> o:A.array UInt32.t
+  -> i:A.array UInt8.t ->
+  RST unit
+    (A.array_resource o <*> A.array_resource i)
+    (fun _ -> A.array_resource o <*> A.array_resource i)
+    (requires fun h0 ->
+      A.vlength o == len /\ A.vlength i == len * 4 /\
+      P.allows_write (A.get_rperm o h0))
+    (ensures  fun h0 _ h1 ->
+      A.vlength o == len /\ A.vlength i == len * 4 /\
+      h0 (A.array_resource i) == h1 (A.array_resource i) /\
+      P.allows_write (A.get_rperm o h1) /\
+      A.as_rseq o h1 == Spec.uints_from_bytes_le (A.as_rseq i h0)
+    )
+
+val uints_to_bytes_le:  #len:nat
+  -> o:A.array UInt8.t{A.vlength o == len * 4}
+  -> i:A.array UInt32.t{A.vlength i == len} ->
+  RST unit
+    (A.array_resource o <*> A.array_resource i)
+    (fun _ -> A.array_resource o <*> A.array_resource i)
+    (requires fun h0 ->
+      P.allows_write (A.get_rperm o h0))
+    (ensures  fun h0 _ h1 ->
+      h0 (A.array_resource i) == h1 (A.array_resource i) /\
+      P.allows_write (A.get_rperm o h1) /\
+      A.as_rseq o h1 == Spec.uints_to_bytes_le (A.as_rseq i h0)
+    )
+
+val xor_block:
+    o:A.array UInt8.t{A.vlength o == 64}
+  -> st:state
+  -> b:A.array UInt8.t{A.vlength b == 64} ->
+  RST unit
+    (A.array_resource o <*> A.array_resource st <*> A.array_resource b)
+    (fun _ -> A.array_resource o <*> A.array_resource st <*> A.array_resource b)
+    (requires fun h ->
+      // TODO: Figure out why is_subresource lemmas patterns are not triggering,
+      // although they are for funcions in Chacha20.fst
+      assert (A.array_resource o `is_subresource_of` (A.array_resource o <*> A.array_resource st));
+      assert ( (A.array_resource o <*> A.array_resource st) `is_subresource_of`
+        (A.array_resource o <*> A.array_resource st <*> A.array_resource b));
+      P.allows_write (A.get_rperm o h))
+    (ensures  fun h0 _ h1 ->
+      assert (A.array_resource o `is_subresource_of` (A.array_resource o <*> A.array_resource st));
+      assert (A.array_resource st `is_subresource_of` (A.array_resource o <*> A.array_resource st));
+      assert ( (A.array_resource o <*> A.array_resource st) `is_subresource_of`
+        (A.array_resource o <*> A.array_resource st <*> A.array_resource b));
+
+      h0 (A.array_resource st) == h1 (A.array_resource st) /\
+      h0 (A.array_resource b) == h1 (A.array_resource b) /\
+      P.allows_write (A.get_rperm o h1) /\
+      A.as_rseq o h1 `Seq.equal` Spec.xor_block (A.as_rseq st h0) (A.as_rseq b h0))
